Backport calling convention requirements to x86 assembly
Now, the requirements on stack pointer and return address,
necessary for the correctness statement of CompCertX, are made
to hold at every external function call in x86 assembly.

Whole-program CompCert still compiles correctly on all 3
architectures, but only x86 can be used with CompCertX.

backend/Asmgenproof0.v
@@ -150,6 +150,7 @@ Qed.
 Record agree (ms: Mach.regset) (sp: val) (rs: Asm.regset) : Prop := mkagree {
   agree_sp: rs#SP = sp;
   agree_sp_def: sp <> Vundef;
+  agree_sp_type: Val.has_type sp Tint;
   agree_mregs: forall r: mreg, Val.lessdef (ms r) (rs#(preg_of r))
 }.
 
@@ -302,6 +303,7 @@ Qed.
 Lemma agree_change_sp:
   forall ms sp rs sp',
   agree ms sp rs -> sp' <> Vundef ->
+  forall TYPE: Val.has_type sp' Tint,
   agree ms sp' (rs#SP <- sp').
 Proof.
   intros. inv H. split; auto.
@@ -864,6 +866,8 @@ Section MATCH_STACK.
 Variables init_sp init_ra: val.
 Hypothesis init_sp_not_vundef: init_sp <> Vundef.
 Hypothesis init_ra_not_vundef: init_ra <> Vundef.
+Hypothesis init_sp_type: Val.has_type init_sp Tint.
+Hypothesis init_ra_type: Val.has_type init_ra Tint.
 
 Variable ge: Mach.genv.
 
@@ -874,6 +878,7 @@ Inductive match_stack: list Mach.stackframe -> Prop :=
       Genv.find_funct_ptr ge fb = Some (Internal f) ->
       transl_code_at_pc ge ra fb f c false tf tc ->
       sp <> Vundef ->
+      forall SP_TYPE: Val.has_type sp Tint,
       match_stack s ->
       match_stack (Stackframe fb sp ra c :: s).
 
@@ -882,6 +887,12 @@ Proof. induction 1; simpl; congruence. Qed.
 
 Lemma parent_ra_def: forall s, match_stack s -> parent_ra init_ra s <> Vundef.
 Proof. induction 1; simpl; try congruence. inv H0. congruence. Qed.
+
+Lemma parent_sp_type: forall s, match_stack s -> Val.has_type (parent_sp init_sp s) Tint.
+Proof. induction 1; simpl; congruence. Qed.
+
+Lemma parent_ra_type: forall s, match_stack s -> Val.has_type (parent_ra init_ra s) Tint.
+Proof. induction 1; simpl; try congruence. inv H0. constructor. Qed.
 
 Lemma lessdef_parent_sp:
   forall s v,
